ldq.lean
@@ -57,8 +57,8 @@ lemma ldq_qfree [atom α β] (qe : list α → fm α)
     apply allp_filter, apply atoms_conj_qfree 
   end
 
-def is_dnf_qe (β : Type) [HA : atom α β] (qe : list α → fm α) (as : list α) : Prop := 
-  ∀ (xs : list β), ((@I _ _ HA (qe as) xs) ↔ (∃ x, (∀ a, a ∈ as → I (A' a) (x::xs))))
+def is_dnf_qe (β : Type) [atom α β] (qe : list α → fm α) (as : list α) : Prop := 
+  ∀ (xs : list β), ((I (qe as) xs) ↔ (∃ x, (∀ a, a ∈ as → I (A' a) (x::xs))))
 
 lemma foo (Q : list β → α → Prop) (a : α) : ∀ (bss : list (list β)), 
   list.map (λ bs, Q bs a) bss = list.map (λ (P : α → Prop), P a) (list.map Q bss)  
@@ -188,7 +188,7 @@ lemma ldq_prsv [HA : atom α β] (qe : list α → fm α)
     apply mem_of_mem_filter,
     apply Ha, rewrite exp_I_list_conj,
     rewrite map_compose, unfold all_true, 
-    intros q Hq, cases (exp_mem_map Hq) with a Ha,
+    intros q Hq, cases (ex_arg_of_mem_map Hq) with a Ha,
     simp at Ha, rewrite Ha^.elim_left, 
     cases H3 with b Hb, unfold I, unfold interp,
     rewrite decr_prsv a _ b, apply Hb, 
